пример:

$$ \frac{1}{625} $$

мой ответ:

$$ \frac{1}{625} = 5^{-1}$$

правильный ответ:

$$ \frac{1}{625} = 5^{-1}$$

пример:

$$ 2^{-2} $$

мой ответ:

$$ 2^{-2} = \frac{1}{4}$$

правильный ответ:

$$ 2^{-2} = \frac{1}{4}$$

правило:

$$ A^{-b} = \frac{1}{A^b}$$

правило:

$$ A^0 = 1 $$

пример:

$$ (\frac{2}{3})^{-2} $$

мой ответ:

$$ (\frac{2}{3})^{-2} = \frac{1}{4/9} = \frac{1}{2^2/3^2}$$

правильный ответ:

$$ (\frac{2}{3})^{-2} = \frac{1}{4/9} = 9:4$$

пример:

$$ (\frac{2}{3})^{-2} $$

мой ответ:

$$ (\frac{2}{3})^{-2} = \frac{1}{4/9} = \frac{1}{2^2/3^2}$$

правильный ответ:

$$ (\frac{2}{3})^{-2} = \frac{1}{4/9} = 9:4 = (\frac{3}{2})^2$$

и к слову вытикает правило:

$$ (\frac{2}{3})^{-2} = (\frac{3}{2})^2$$

просто перевернув дробь с отрицателной степенью мы превратили ее в положительную:

$$ (\frac{A}{B})^{-n} = (\frac{B}{A})^n$$

пример:

$$ 0.3^{-2} $$

мой ответ:

$$ 0.3^{-2} = (\frac{1}{0.3^2}) $$

правильный ответ:

$$ 0.3^{-2} = (\frac{3}{10})^{-2} = (\frac{10}{3})^2$$
