пример:

$$ A^{-5} $$

мой ответ:

$$ A^{-5} = \frac{1}{A^5}$$

правильный ответ:

$$ A^{-5} = \frac{1}{A^5}$$

пример:

$$ 2X^{-4} $$

мой ответ:

$$ 2X^{-4} = \frac{1}{2 × X^4}$$

правильный ответ:

$$ 2X^{-4} = \frac{2}{X^4}$$

пример:

$$ 5(XY)^{-3} $$

мой ответ:

$$ 5(XY)^{-3} = \frac{5}{X^3 × Y^3}$$

правильный ответ:

$$ 5(XY)^{-3} = \frac{5}{X^3 × Y^3}$$

пример:

$$ \frac{1}{A^9} $$

мой ответ:

$$ \frac{1}{A^9} = A^{-9}$$

правильный ответ:

$$ \frac{1}{A^9} = A^{-9}$$

пример:

$$ \frac{6}{X^{-4}} $$

мой ответ:

$$ \frac{6}{X^{-4}} = \frac{6}{\frac{1}{X^9}}$$

правильный ответ:

$$ \frac{6}{X^{-4}} = 6 × X^4$$

пример:

$$ 7^{-4} × 7^6$$

мой ответ:

$$ 7^{-4} × 7^6 = 7^2 = 49$$

правильный ответ:

$$ 7^{-4} × 7^6 = 7^2 = 41$$

пример:

$$ 2^2 : 2^{-3} $$

мой ответ:

$$ 2^2 : 2^{-3} = 2^5$$

правильный ответ:

$$ 2^2 : 2^{-3} = 2^5$$

пример:

$$ 8^{-2} : 4^3 $$

мой ответ:

$$ 8^{-2} : 4^3 = \frac{4^3 = 16 × 4}{8^2 = 8 × 8} = 1$$

правильный ответ:

$$ 8^{-2} : 4^3 = 2^{-12} $$
