пример:

$$ 18 × (-9)^{-1} $$

мой ответ:

$$ 18 × (-9)^{-1} = 18 × \frac{1}{-9}$$

правильный ответ:

$$ 18 × (-9)^{-1} = -2$$

пример:

$$ 0.5^{-2} + (\frac{1}{4})^{-1} $$

мой ответ:

$$ 0.5^{-2} + (\frac{1}{4})^{-1} = \frac{1}{\frac{1}{4}} + (\frac{4}{1})^{1} = 4 + 4 = 8$$

правильный ответ:

$$ 0.5^{-2} + (\frac{1}{4})^{-1} = (\frac{5}{10})^{-2} + (\frac{1}{4})^{-1} = 4 + 4 = 8$$

пример:

$$ (\frac{X^{-3} × Y^4}{9})^{-2} × (\frac{3}{X^{-2} × Y^3})^{-4}$$

мой ответ:

$$
(\frac{X^{-3} × Y^4}{9})^{-2} × (\frac{3}{X^{-2} × Y^3})^{-4}
= (\frac{9}{X^{-3} × Y^4})^2 × (\frac{X^{-2} × Y^3}{3})^4
= (\frac{9^2}{X^{-3 × 2} × Y^{4 × 2}}) × (\frac{X^{-2 × 4} × Y^{3 × 4}}{3^4})
= (\frac{9^2}{X^{-6} × Y^{8}}) × (\frac{X^{-8} × Y^{12}}{3^4})
= \frac{81}{X^{-6} × Y^{8}} × \frac{X^{-8} × Y^{12}}{81}
= \frac{81}{X^{-6} × Y^{8}} : \frac{81}{X^{-8} × Y^{12}}
= \frac{1}{X^{-6 - -8} × Y^{8-12}}
= \frac{1}{X^{-6+8} × Y^{-4}}
= \frac{1}{X^{2} × Y^{-4}}
= \frac{1}{X^{2} × (1/Y^4)}
$$

правильный ответ:

$$ (\frac{X^{-3} × Y^4}{9})^{-2} × (\frac{3}{X^{-2} × Y^3})^{-4} = много ответов $$

пример: Докажи

$$ 3 × 2^n + 2^n = 2^{n+2}$$

мой ответ:

$$ 3 × 2^n + 2^n = 2^{n+2} = 4× 2^n = 2^{n+2} = 2^2 × 2^n = 2^{n+2} = 2^{n+2}$$
если подставить к n 1
$$ 3 × 2^1 + 2^1 = 2^{1+2} = 4 × 2^1 = 2^{1+2} = 8 = 8$$

правильный ответ:

$$ 3 × 2^n + 2^n = 2^{n+2} = $$
