пример:

$$ (0.25 × A^{-4} × X^{-3})^2 × (\frac{A^{-3}}{4 × X^2})^{-3} $$

мой ответ:

$$
(0.25 × A^{-4} × X^{-3})^2 × (\frac{A^{-3}}{4 × X^2})^{-3}
= 0.25 × A^{-8} × X^{-6} × \frac{A^9}{4 × X^{-6}}
= 0.25 × (1:(A^8)) × (1:(X^6)) × \frac{A^9}{4 × (1:(X^6))}
= (1:(A^8 × 4)) × (1:(X^6)) × \frac{A^9}{4:(X^6)}
= (1:(X^6 × (4 × A^8))) × \frac{A^9}{4:(X^6)}
= \frac{1}{X^6 × (4 × A^8)} × \frac{A^9}{4:(X^6)}
= \frac{A^9}{X^6 × (4:(X^6)) × (4 × A^8)}
= \frac{A^9}{\frac{X^6 × 4}{2 × X^6} × (4 × A^8)}
= \frac{A^9}{\frac{X^6 × 2}{X^6} × (4 × A^8)}
= \frac{A^9}{2 × (4 × A^8)}
= \frac{A^9}{8A^8}
= \frac{A}{7A^8}
$$

правильный ответ:

$$ (0.25 × A^{-4} × X^{-3})^2 × (\frac{A^{-3}}{4 × X^2})^{-3} = $$

пример:

$$ \frac{12^n}{2^{2n-1} × 3^{n+1}} $$

мой ответ:

$$
\frac{12^n}{2^{2n-1} × 3^{n+1}}
= \frac{(2^2)^n × 3^n}{2^{2n-1} × 3^{n+1}}
= \frac{(2^2)^n × 3^n}{(2^2)^{(n-1)} × 3^{n+1}}
= 2 × 3^{-1}
= 2/3
$$

праивльный ответ:

$$ \frac{12^n}{2^{2n-1} × 3^{n+1}} = 2/3$$

пример:

$$ \frac{45^{n+1}}{3^{2n+1} × 5^n} $$

мой ответ:

$$
\frac{45^{n+1}}{3^{2n+1} × 5^n}
= \frac{3^{n+1} × 3^{n+1} × 5^{n+1}}{3^{2n+1} × 5^n}
= \frac{3^{n+1} × 3^{n+1} × 5^1}{3^{2n+1}}
= \frac{3^{2n+2} × 5}{3^{2n+1}}
= 3 × 5
= 15
$$

праивльный ответ:

$$ \frac{45^{n+1}}{3^{2n+1} × 5^n} = $$
