Раньше мы Из Скобочки в Формулу превращяли а теперь наоборот:

`9a^2 - 24ab + 16b^2` = `(3a)^2 - (2 × 3a × 4b) + (4b)^2` = `(3a - 4b)^2`

`100a^2 + 20ab + b^2` = `(10a)^2 + (2 × 10a × 1b) + b^2` = `10a + b`

`10mn + 100m^2 + 0.25n^2` = `100m^2 + 10mn + 0.25n^2` = `(10m)^2 + 10mn + (0.5n)^2` = `(10m)^2 + 2 × 10m × 0.5n + (0.5n)^2` = `(10m + 0.5n)^2`

`100a^2 + 60ab + 9b^2`, если `a = 0.8` а `b = -3`. сокращяем вырожение: `(10a)^2 + 60ab + (3b)^2` = `(10a)^2 + 2 × 10a × 3b + (3b)^2` = `(10a + 3b)^2`

подсовляем: `(10a + 3b)^2` = `(10 × 0.8 + 3 × -3)^2` = `(8 + -9)^2` = `(-1)^2` = `1`
