$$ (-2 + x)(2 + x) = (x - 2)(x + 2) = x^2 - 2^2 = x^2 - 4 $$

$$ (-2ab + c)(c + 2ab) = (c - 2ab)(c + 2ab) = c^2 - (2ab)^2 $$

$$ (5m - 1/2p)(5m + 1/2p) = (5m)^2 - (1/2p)^2 = 25m^2 - 0.25p^2 $$

$$ (4 - 3xy)(4 + 3xy) = 4^2 - (3xy)^2 $$

тут уже нельзя зделать все по формуле мы посто вычисляем:

$$ (5 - x)(2 + x) = 5 × 2 + 5 × x + -x × 2 + -x × x = 10 + 5x + -2x + -x^2 = 10 + 5x - 2x - x^2 = 10 + 3x - x^2 $$

$$ 36p^2 - 25q^2 = (6p - 5q)(6p + 5q) $$

$$ 1 - 64a^8 = 1^2 - (8a^4)^2 = (1 - 8a^4)(1 + 8a^4) $$

$$ \frac{a^4b^6}{9} - \frac{c^y}{16} $$
