$$ (a + 2)^2 - 1 = (a + 2)(a + 2) - 1 = a × a + a × 2 + 2 × a + 2^2 - 1 = a^2 + 2a2 + 2^2 - 1 = a^2 + 4a + 4 - 1 = a^2 + 4a + 3 $$

но ведь можно и точно также:

$$ (a + 2)^2 - 1^2 $$

и тут вы поняли `(a + 2)^2` это `a^2`, а `1^2` это `b^2` и между ними минус! а значит Формула Пременима:

$$ (a + 2)^2 - 1^2 = (a + b - 1)(a + b + 1) $$

$$ 16 - (x + y)^2 = 4^2 - (x + y)^2 = (4 - x + y)(4 + x + y) $$

$$ (2a + 5)^2 - 49 = (2a + 5)^2 - 7^2 = (2a + 5 - 7)(2a + 5 + 7) = (2a - 2)(2a + 12) $$

$$ (x^n + y^n)(x^n - y^n) = x^2n - y^2n $$

$$ (a - 2)(a + 2)(a^2 + 4) = (a^2 - 2^2)(a^2 + 4) = (a^2 - 2^2)(a^2 + 2^2) = a^2^2 - 2^2^2 = a^4 - 2^4 = a^4 - 16 $$
