$$
(2a + b)^2 - (a - 2b)^2
= (2a + b - (a - 2b))(2a + b + a - 2b)
= (2a + b + -a + 2b)(2a + b + a - 2b)
= (2a + b - a + 2b)(2a + b + a - 2b)
= (a + 3b)(3a - b)
$$

$$
x^6 - (2y^2 - x^3)^2
= (x^3 - (2y^2 - x^3))(x^3 + (2y^2 - x^3))
= (x^3 + -2y^2 + x^3)(x^3 + 2y^2 - x^3)
= (x^3 - 2y^2 + x^3)(x^3 + 2y^2 - x^3)
= (2x^3 - 2y^2)(2y^2)
$$

$$ \frac{92^2 - 48^2}{27^2 - 17^2} = (92 - 48)(92 + 48)/(27 - 17)(27 + 17) = (44)(140)/(10)(44) = 14 $$

$$ 2.1 Ã— 1.9 = (2 - 0.1)(2 + 0.1) = 2^2 - 0.1^2 = 4 - 0.1 = 3.99 $$
