$$
(a + b)(a^2 - ab + b^2)
= a^3 - a × ab + ab^2 + ba^2 - bab + b^3
= a^3 - a^2b + ab^2 + a^2b - ab^2 + b^3
= a^3 + b^3
$$

итого новая формула: `(a + b)(a^2 - ab + b^2) = a^3 + b^3`
и еще формула: `(a - b)(a^2 + ab + b^2) = a^3 - b^3`

$$ m^3 - n^3 = (m - n)(m^2 + mn + n^2) $$

$$ a^3 - 8 = a^3 - 2^3 = (a + 2)(a^2 - a2 + 2^2) = (a + 2)(a^2 - 2a + 4) $$

$$ 27 - 64a = 3^3 - (4a)^3 = (3 - 4a)(3^2 + 3a4 + (4a)^2) = (3 - 4a)(9 + 12a + 16a^2) = $$

$$ (x + 2y)(x^2 - 2xy + 4y^2) = x^3 + (2y)^3 = x^3 + 8y^3 $$
