$$ \frac{15x(y + 2)}{6y + 12} = \frac{15x(y + 2)}{6(y + 2)} = \frac{15x(y + 2)}{6(y + 2)} = \frac{15x}{6} = \frac{5 × 3 × x}{2 × 3} = \frac{5x}{2} $$

$$ \frac{x^2 - 9}{3x - 9} = \frac{x^2 - 9}{3(x - 3)} = \frac{x^2 - 3^2}{3(x - 3)} = \frac{(x - 3)(x + 3)}{3(x - 3)} = \frac{x + 3}{3} $$

$$ \frac{6xy - 18x^2}{(y - 3x)^3} = \frac{6x(y - 3x)}{(y - 3x)(y - 3x)(y - 3x)} = \frac{6x}{(y - 3x)(y - 3x)} = \frac{6x}{(y - 3x)^2} $$

$$ \frac{a^3 - b^3}{a - b} = \frac{(a - b)(a^2 + 2ab + b^2)}{a - b} \frac{(a - b)(a^2 + 2ab + b^2)}{(a - b) × 1} = \frac{a^2 + 2ab + b^2}{1} = a^2 + 2ab + b^2 $$
