$$
\frac{3a^2 - 6ab + 3b^2}{6a^2 - 6b^2}
= \frac{3(a^2 - 2ab + b^2)}{6(a^2 - b^2)}
= \frac{a^2 - 2ab + b^2}{2(a^2 - b^2)}
= \frac{(a - b)^2}{2(a^2 - b^2)}
= \frac{(a - b)^2}{2(a - b)(a + b)}
= \frac{(a - b)(a - b)}{2(a - b)(a + b)}
= \frac{(a - b)}{2(a + b)}
$$

$$
\frac{1 - 2x + x^2}{x^2 - 1}
= \frac{1^2 - 2x + x^2}{x^2 - 1^2}
= \frac{(1 - x)^2}{(x + 1)(x - 1)}
= \frac{(1 - x)^2}{(x + 1)(x - 1)}
= \frac{ - (x - 1)^2}{(x + 1)(x - 1)}
= \frac{ -(x - 1) × -(x - 1)}{(x + 1)(x - 1)}
= \frac{(x - 1) × (x - 1)}{(x + 1)(x - 1)}
= \frac{(x - 1)}{(x + 1)}


$$

$$
\frac{ax + ay - bx - by}{ax - ay - bx + by}
= \frac{(ax + ay) - (bx + by)}{(ax - ay) - (bx - by)}
= \frac{a(x + y) - b(x + y)}{a(x - y) - b(x - y)}
= \frac{(a - b)(x + y)}{(a - b)(x - y)}
= \frac{x + y}{x - y}


$$ \frac{2p^2 - 3qp}{8p^3 - 27q^3 + 54pq^2 - 36pq^2} $$

при `q = 2/3`, `p = 1/2`. мы помним что надо `упростить` а потом `подставим`


$$

\frac{2p^2 - 3qp}{8p^3 - 36qp^2 + 54pq^2 - 27q^3}
= \frac{p(2p - 3q)}{(2p)^3 - 36qp^2 + 54pq^2 - (3q)^3}
= \frac{p(2p - 3q)}{(2p - 3q)^3}
= \frac{p}{(2p - 3q)^2}$$

а теперь подстовляем:

$$ \frac{p}{(2p - 3q)^2} = \frac{1/2}{(2 × 1/2 - 3 × 2/3)^2} = \frac{1/2}{(1 - 6/3)^2} = \frac{1/2}{(1 - 2)^2} = \frac{1/2}{(-1)^2} = \frac{1/2}{1} = 1/2 $$
