что бы суммировать дробь с Одинаковами Знаминателями надо `(a)/c + (b)/c = (a) + (b)/c`

$$
\frac{ax - y}{a + b} + \frac{y + bx}{a + b}
= \frac{ax - y + y + bx}{a + b}
= \frac{ax + bx}{a + b}
= \frac{x(a + b)}{a + b}
= x
$$

$$
\frac{x + 2}{c^2 - 3} - \frac{x - 3}{c^2 - 3}
= \frac{x + 2 - (x - 3)}{c^2 - 3}
= \frac{x + 2 - x + 3}{c^2 - 3}
= \frac{5}{c^2 - 3}
$$

$$
\frac{2x + b}{x - y} + \frac{3x + b}{y - x}
= \frac{2x + b}{x - y} - \frac{3x + b}{x - y}
= \frac{2x + b - (3x + b)}{x - y}
= \frac{2x + b - 3x - b}{x - y}
= \frac{-x}{x - y}
= -\frac{x}{x - y}
= -\frac{x}{-(y - x)}
= \frac{x}{y - x}
$$

$$
\frac{x + 1}{a - b} - \frac{x + 2}{b - a} - \frac{x - 1}{a - b}
= \frac{x + 1}{a - b} + \frac{x + 2}{a - b} - \frac{x - 1}{a - b}
= \frac{x + 1 + (x + 2) - (x - 1)}{a - b}
= \frac{x + 1 + x + 2 - (x - 1)}{a - b}
= \frac{2x + 3 - (x - 1)}{a - b}
= \frac{2x + 3 - x + 1}{a - b}
= \frac{x + 4}{a - b}
$$
