$$
\frac{c}{12b} + \frac{1}{4b^4}
= \frac{c}{3 × 4 × b} + \frac{1}{4 × b × b^3}
= \frac{(c × b^3) + (1 × 3)}{3 × 4 × b × b^3}
= \frac{cb^3 + 3}{12b^4}
= \frac{cb^3 + 3}{12b^4}
$$

итак а если не `1/3z - 1/2z` а `1/z + 1 - 1/z + 1` то тогда `1/(z + 1)(z + 1)`

$$
\frac{1}{z - 3} - \frac{1}{z + 3}
= \frac{1(z + 3) - 1(z - 3)}{(z - 3)(z + 3)}
= \frac{z + 3 - z + 3}{(z - 3)(z + 3)}
= \frac{6}{(z - 3)(z + 3)}
= \frac{6}{z^2 - 3^2}
= \frac{6}{z^2 - 9}
$$

$$
\frac{x + 3}{x^2 + xy} - \frac{y - 3}{y^2 + xy}
= \frac{x + 3}{x(x + y)} - \frac{y - 3}{y(y + x)}
= \frac{y(x + 3) - x(y - 3)}{x(x + y)y(y + x)}
= \frac{y(x + 3) - x(y - 3)}{(x + y)(x + y)}
= \frac{xy + 3y - xy + 3x}{(x + y)(x + y)}
= \frac{3y + 3x}{(x + y)(x + y)}
= \frac{3(y + x)}{(x + y)(x + y)}
= \frac{3}{x + y}
$$
