$$
\frac{3}{x - 3} - \frac{x + 15}{x^2 - 9} - \frac{2}{x}
= \frac{3}{x - 3} - \frac{x + 15}{x × x - 3 × 3} - \frac{2}{x}
$$

но учитель делает так:

$$
\frac{3}{x - 3} - \frac{x + 15}{x^2 - 9} - \frac{2}{x}
= \frac{3}{x - 3} - \frac{x + 15}{x^2 - 3^2} - \frac{2}{x}
= \frac{3}{x - 3} - \frac{x + 15}{(x - 3)(x + 3)} - \frac{2}{x}
= \frac{(3 × x(x + 3)) - (x + 15 × x) - (2 × (x - 3)(x + 3))}{(x - 3)(x + 3)x}
= \frac{3x(x + 3) - x(x + 15) - 2(x^2 - 9)}{(x - 3)(x + 3)x}
= \frac{3x × x + 3x × 3 - x × x - x × 15 - 2 × x^2 + 2 × 9}{(x - 3)(x + 3)x}
= \frac{3x^2 + 9x - x^2 - 15x - 2x^2 + 18}{(x - 3)(x + 3)x}
= \frac{-6x + 18}{(x - 3)(x + 3)x}
= \frac{18 - 6x}{(x - 3)(x + 3)x}
= \frac{6(3 - x)}{(x - 3)(x + 3)x}
= \frac{-6(x - 3)}{(x - 3)(x + 3)x}
= \frac{-6}{x(x + 3)}
$$

$$
\frac{2a^2 - a}{a^3 + 1} - \frac{a - 1}{a^2 - a + 1}
= \frac{2a^2 - a}{a^3 + 1^3} - \frac{a - 1}{a^2 - a + 1}
= \frac{2a^2 - a}{(a + 1)(a^2 - a1 + 1^2)} - \frac{a - 1}{a^2 - a1 + 1^2}
= \frac{(2a^2 - a) - (a + 1)(a - 1)}{(a + 1)(a^2 - a1 + 1^2)}
= \frac{(2a^2 - a) - (a^2 - 1^2)}{(a + 1)(a^2 - a1 + 1^2)}
= \frac{2a^2 - a - a^2 + 1}{(a + 1)(a^2 - a1 + 1^2)}
= \frac{a^2 - a + 1}{(a + 1)(a^2 - a1 + 1^2)}
= \frac{1}{a + 1}
$$
