$$
\frac{6yx^2}{x^2 - xy + y^2} + \frac{6xy}{x + y} - \frac{12yx^3}{x^3 + y^3}
= \frac{6yx^2}{(x - y)^2} + \frac{6xy}{x + y} - \frac{12yx^3}{(x + y)(x^2 - xy + y^2)}
$$

но учитель делает так:

$$
\frac{6yx^2}{x^2 - xy + y^2} + \frac{6xy}{x + y} - \frac{12yx^3}{x^3 + y^3}
= \frac{6yx^2}{x^2 - xy + y^2} + \frac{6xy}{x + y} - \frac{12yx^3}{(x + y)(x^2 - xy + y^2)}
= \frac{(6yx^2 × (x + y)) + (6xy × (x^2 - xy + y^2)) - (12yx^3)}{(x + y)(x^2 - xy + y^2)}
= \frac{6yx^2(x + y) + 6xy(x^2 - xy + y^2) - 12yx^3}{(x + y)(x^2 - xy + y^2)}
= \frac{6yx^2(x + y) + 6xy × x^2 -  6xy × xy + 6xy × y^2 - 12yx^3}{(x + y)(x^2 - xy + y^2)}
= \frac{6yx^2(x + y) + 6xyxx - 6xyxy + 6xyyy - 12yx^3}{(x + y)(x^2 - xy + y^2)}
= \frac{6yx^2 × x + 6yx^2 × y + 6xyxx - 6xyxy + 6xyyy - 12yx^3}{(x + y)(x^2 - xy + y^2)}
= \frac{6yx^3 + 6yyx^2 + 6yxxx - 6yyxx + 6xyyy - 12yx^3}{(x + y)(x^2 - xy + y^2)}
= \frac{6yx^3 + 6 × y^2 × x^2 + 6yx^3 - 6 × y^2 × x^2 + 6xy^3 - 12yx^3}{(x + y)(x^2 - xy + y^2)}
= \frac{6yx^3 + 6yx^3 - 12yx^3 + 6 × y^2 × x^2 - 6 × y^2 × x^2 + 6xy^3}{(x + y)(x^2 - xy + y^2)}
= \frac{6xy^3}{(x + y)(x^2 - xy + y^2)}
= \frac{6xy^3}{x^3 + y^3}
$$

$$
\frac{1}{2x + 2} - \frac{x - 1}{3x^2 + 6x + 3}
= \frac{1}{2 × x + 2} - \frac{x - 1}{3 × x × x + 2 × 3 × x + 3}
$$

но учитель делает так:

$$
\frac{1}{2x + 2} - \frac{x - 1}{3x^2 + 6x + 3}
= \frac{1}{2(x + 1)} - \frac{x - 1}{3(x^2 + 2x + 1)}
= \frac{1}{2(x + 1)} - \frac{x - 1}{3(x^2 + 2x1 + 1^2)}
= \frac{1}{2(x + 1)} - \frac{x - 1}{3(x + 1)^2}
= \frac{1}{2(x + 1)} - \frac{x - 1}{3(x + 1)(x + 1)}
= \frac{3(x + 1) - 2(x - 1)}{3(x + 1)(x + 1)2}
= \frac{3x + 3 - 2x + 2}{3(x + 1)(x + 1)2}
= \frac{x + 5}{3(x + 1)(x + 1)2}
= \frac{x + 5}{6(x + 1)(x + 1)}
$$
