$$ \frac{a}{b} × \frac{c}{d} = \frac{a × c}{b × d} $$

$$ \frac{a}{b} / \frac{c}{d} = \frac{a}{b} × \frac{d}{c} = \frac{a × d}{b × c} $$

$$
\frac{48a^4}{49b^4} × \frac{7b^2}{16a^2}
= \frac{336 × a^4 × b^2}{784 × b^4 × a^2}
= \frac{3 × a^4 × b^2}{7 × b^4 × a^2}
= \frac{3}{7}a^2 × b^{-2}
= \frac{3a^2}{7b^2}
$$

$$
\frac{a^2 - b^2}{6 × a^2 × b^2} / \frac{a + b}{3ab}
= \frac{a^2 - b^2}{6 × a^2 × b^2} × \frac{3ab}{a + b}
= \frac{3ab(a^2 - b^2)}{(a + b)(6 × a^2 × b^2)}
= \frac{ab(a^2 - b^2)}{(a + b)(2 × a^2 × b^2)}
= \frac{ab(a - b)(a + b)}{(a + b)(2 × a^2 × b^2)}
= \frac{ab(a - b)}{2 × a^2 × b^2}
= \frac{ab(a - b)}{2 × aa × bb}
= \frac{a - b}{2 × a × b}
$$

$$ \frac{3ab}{6× a^2 × b^2} = \frac{ab}{2 × a^2 × b^2} = \frac{1}{2ab} $$
