$$
\frac{a^2 × b - 4 × b^3}{3ab^3} × \frac{a^2 × b}{a^2 - 2ab}
= \frac{(a^2 × b - 4 × b^3) × (a^2 × b)}{(3ab^3) × (a^2 - 2ab)}
= \frac{(aab - 4bbb) × (aab)}{(3abbb) × (aa - 2ab)}
= \frac{b(aa - 4bb) × aab}{3abbb × a(a - 2b)}
= \frac{a(aa - 4bb)}{3b × a(a - 2b)}
= \frac{a(aa - 4bb)}{3ab(a - 2b)}
= \frac{a^2 - 4b^2}{3b(a - 2b)}
= \frac{(a - 2b)^2}{3b(a - 2b)}
= \frac{(a - 2b)^2}{3b(a - 2b)}
= \frac{(a - 2b)(a - 2b)}{3b(a - 2b)}
= \frac{a - 2b}{3b}
$$

$$
\frac{3x^2 - 3y^2}{a^2 + ax} / \frac{6x - 6y}{x + a}
= \frac{3x^2 - 3y^2}{a^2 + ax} × \frac{x + a}{6x - 6y}
= \frac{(3x^2 - 3y^2) × (x + a)}{(a^2 + ax) × (6x - 6y)}
= \frac{(3xx - 3yy) × (x + a)}{(aa + ax) × (6x - 6y)}
= \frac{3(xx - yy) × (x + a)}{a(a + x) × 6(x - y)}
= \frac{3(xx - yy) × (x + a)}{a(x + a) × 6(x - y)}
= \frac{3(xx - yy)}{a × 6(x - y)}
= \frac{3(xx - yy)}{6a(x - y)}
= \frac{xx - yy}{2a(x - y)}
= \frac{x^2 - y^2}{2a × (x - y)}
= \frac{x - y}{2a}
$$

$$
\frac{4x^2 - 25y^2}{x^3 + 8} / \frac{2x + 5y}{x^2 - 2x + 4}
= \frac{4x^2 - 25y^2}{x^3 + 2^3} / \frac{2x + 5y}{x^2 - 2x + 2^2}
= \frac{4x^2 - 25y^2}{x^3 + 2^3} × \frac{x^2 - 2x + 2^2}{2x + 5y}
= \frac{(4x^2 - 25y^2) × (x^2 - 2x + 2^2)}{(x^3 + 2^3) × (2x + 5y)}
= \frac{((2x)^2 - (5y)^2) × (x - 2)^2}{(x^3 + 2^3) × (2x + 5y)}
= \frac{(2x - 5y)(2x + 5y) × (x - 2)^2}{(x^3 + 2^3) × (2x + 5y)}
= \frac{(2x - 5y)(x - 2)(x - 2)}{(x^3 + 2^3)}
$$

учитель делает проще и эффектнее:

$$
\frac{4x^2 - 25y^2}{x^3 + 8} / \frac{2x + 5y}{x^2 - 2x + 4}
= \frac{4x^2 - 25y^2}{x^3 + 2^3} / \frac{2x + 5y}{x^2 - 2x + 2^2}
= \frac{4x^2 - 25y^2}{x^3 + 2^3} × \frac{x^2 - 2x + 2^2}{2x + 5y}
= \frac{(2x)^2 - (5y)^2}{x^3 + 2^3} × \frac{x^2 - 2x + 2^2}{2x + 5y}
= \frac{(2x - 5y)(2x + 5y)}{x^3 + 2^3} × \frac{x^2 - 2x + 2^2}{2x + 5y}
= \frac{(2x - 5y)(2x + 5y)}{(x + 2)(x^2 - 2x + 2^2)} × \frac{x^2 - 2x + 2^2}{2x + 5y}
$$

а я продолжаю мысль учителя:

$$
\frac{(2x - 5y)(2x + 5y)}{(x + 2)(x^2 - 2x + 2^2)} × \frac{x^2 - 2x + 2^2}{2x + 5y}
= \frac{(2x - 5y)}{(x + 2)(x^2 - 2x + 2^2)} × \frac{x^2 - 2x + 2^2}{1}
= \frac{(2x - 5y)}{(x + 2)} × \frac{1}{1}
= \frac{2x - 5y}{x + 2}
$$

$$
\frac{a^2 + ax + ab + bx}{a^2 - ax - ab + bx} × \frac{a^2 - ax - bx + ab}{a^2 + ax - bx - ab}
= \frac{(a^2 + ax + ab) + bx}{(a^2 - ax - ab) + bx} × \frac{a^2 - ax - bx + ab}{a^2 + ax - bx - ab}
= \frac{a(a + x + b) + bx}{a(a - x - b) + bx} × \frac{a^2 - ax - bx + ab}{a^2 + ax - bx - ab}
= \frac{a + x + b + bx}{a - x - b + bx} × \frac{a^2 - ax - bx + ab}{a^2 + ax - bx - ab}
= \frac{a + x + b + bx}{a - x - b + bx} × \frac{a(a - x) - bx + ab}{a(a + x) - bx - ab}
= \frac{a + x + b + bx}{a - x - b + bx} × \frac{a - x - bx + ab}{a + x - bx - ab}
= \frac{(a + x) + b + bx}{a - x - b + bx} × \frac{a - x - bx + ab}{(a + x) - bx - ab}
= \frac{+ b + bx}{a - x - b + bx} × \frac{a - x - bx + ab}{- bx - ab}
= \frac{b + bx}{(a - x) - b + bx} × \frac{(a - x) - bx + ab}{-bx - ab}
= \frac{b + bx}{- b + bx} × \frac{- bx + ab}{-bx - ab}
= \frac{b + bx}{-b + bx} × \frac{-bx + ab}{-bx - ab}
= \frac{b + bx}{bx - b} × \frac{ab - bx}{-bx - ab}
= \frac{b(1 + x)}{b(x - 1)} × \frac{ab - bx}{-bx - ab}
= \frac{1 + x}{x - 1} × \frac{ab - bx}{-bx - ab}
= \frac{1 + x}{x - 1} × \frac{b(a - x)}{b(-x - a)}
= \frac{1 + x}{x - 1} × \frac{a - x}{-x - a}
= \frac{1 + x}{x - 1} × \frac{a - x}{-x - a}
$$
