$$
\frac{a - 2}{4a^2 + 16a + 16} / (\frac{a}{2a - 4} - \frac{a^2 + 4}{2a^2 - 8} - \frac{2}{a^2 + 2a})
= \frac{a - 2}{4a^2 + 16a + 16} / (\frac{a}{2(a - 2)} - \frac{a^2 + 4}{2(a^2 - 2^2)} - \frac{2}{a(a + 2)})
= \frac{a - 2}{4a^2 + 16a + 16} / (\frac{a}{2(a - 2)} - \frac{a^2 + 4}{2(a - 2)(a + 2)} - \frac{2}{a(a + 2)})
= \frac{a - 2}{4a^2 + 16a + 16} / (\frac{a}{2(a - 2)} - \frac{a^2 + 2^2}{2(a - 2)(a + 2)} - \frac{2}{a(a + 2)})
= \frac{a - 2}{4a^2 + 16a + 16} / (\frac{(a × a × (a + 2)) - (a × (a^2 + 2^2)) - (2 × 2 × (a - 2))}{2(a - 2)(a + 2)a})
= \frac{a - 2}{4a^2 + 16a + 16} / (\frac{a^2(a + 2) - a(a^2 + 2^2) - 4(a - 2)}{2(a - 2)(a + 2)a})
= \frac{a - 2}{4a^2 + 16a + 16} / (\frac{(a^3 + 2a^2) - (a^3 + a2^2) - 4(a - 2)}{2(a - 2)(a + 2)a})
= \frac{a - 2}{4a^2 + 16a + 16} / (\frac{(a^3 + 2a^2) - (a^3 + a2^2) - (4a - 8)}{2(a - 2)(a + 2)a})
= \frac{a - 2}{4a^2 + 16a + 16} / (\frac{a^3 + 2a^2 - a^3 - a2^2 - 4a + 8}{2(a - 2)(a + 2)a})
= \frac{a - 2}{4a^2 + 16a + 16} / (\frac{aaa + 2aa - aaa - 4a - 4a + 8}{2(a - 2)(a + 2)a})
= \frac{a - 2}{4a^2 + 16a + 16} / (\frac{2aa - 8a + 8}{2(a - 2)(a + 2)a})
= \frac{a - 2}{4a^2 + 16a + 16} / (\frac{2a^2 - 8a + 8}{2(a - 2)(a + 2)a})
= \frac{(a - 2)(2a(a - 2)(a + 2))}{(4a^2 + 16a + 16)(2a^2 - 8a + 8)}
= \frac{(a - 2)(2a(a - 2)(a + 2))}{(4aa + 16a + 16)(2aa - 8a + 8)}
= \frac{(a - 2)(2a(a - 2)(a + 2))}{2(2aa + 8a + 8)(aa - 4a + 4)}
= \frac{(a - 2)(2a(a - 2)(a + 2))}{2(2aa + 8a + 8)(a^2 - 2 × 2 × a + 2^2)}
= \frac{(a - 2)(2a(a - 2)(a + 2))}{2 × (2(a^2 + 2 × 2 × a + 2^2) × (a - 2)^2)}
= \frac{(a - 2)(2a(a - 2)(a + 2))}{2 × (2(a + 2)^2 × (a - 2)^2)}
= \frac{(a - 2)(2a(a - 2)(a + 2))}{2(2((a + 2)(a + 2)) × (a - 2)(a - 2))}
= \frac{(a - 2)(a(a + 2))}{4(a + 2)(a + 2) × (a - 2)}
= \frac{a(a - 2)}{4(a + 2) × (a - 2)}
= \frac{a}{4(a + 2)}
$$

$$
\frac{a - 2}{4a^2 + 16a + 16} / \frac{a - 2}{a(a + 2)}
= \frac{a - 2}{4a^2 + 16a + 16} × \frac{a(a + 2)}{a - 2}
= \frac{1}{4a^2 + 16a + 16} × \frac{a(a + 2)}{1}
= \frac{a(a + 2)}{4a^2 + 16a + 16}
= \frac{a(a + 2)}{4aa + 16a + 16}
= \frac{a(a + 2)}{4(aa + 4a + 4)}
= \frac{a(a + 2)}{4(a^2 + 2 × 2 × a + 2^2)}
= \frac{a(a + 2)}{4 × (a + 2)^2}
= \frac{a(a + 2)}{4 × (a + 2)(a + 2)}
= \frac{a}{4(a + 2)}
$$
