$$
(\frac{x}{y^2} - \frac{1}{x}) / (\frac{1}{y} + \frac{1}{x})
= (\frac{x}{y^2} - \frac{1}{x}) / \frac{x + y}{xy}
= (\frac{x}{y^2} - \frac{1}{x}) × \frac{xy}{x + y}
= \frac{x(x) - y^2(1)}{xy^2} × \frac{xy}{x + y}
= \frac{x^2 - y^2}{xy^2} × \frac{xy}{x + y}
= \frac{(x - y)(x + y)}{xy^2} × \frac{xy}{x + y}
= \frac{(x - y)(x + y) × xy}{xy^2 × (x + y)}
= \frac{(x - y)(x + y)}{y × (x + y)}
= \frac{x - y}{y}
$$

$$
\frac{ab + b^2}{3} / \frac{b^3}{3a} + \frac{a + b}{b}
= \frac{ab + b^2}{3} × \frac{3a}{b^3} + \frac{a + b}{b}
= \frac{(ab + b^2) × 3a}{3b^3} + \frac{a + b}{b}
= \frac{3a(ab + b^2)}{3b^3} + \frac{a + b}{b}
= \frac{3aab + 3abb}{3bbb} + \frac{a + b}{b}
= \frac{3b(aa + ab)}{3b(bb)} + \frac{a + b}{b}
= \frac{(aa + ab) + b(a + b)}{bb}
= \frac{a(a + b) + b(a + b)}{bb}
= \frac{(a + b)(a + b)}{bb}
= \frac{(a + b)^2}{b^2}
= (\frac{a + b}{b})^2
$$
