$$ x^4 + x^3 + x^2 + x = 9 $$

чему равно:

$$ x^5 - 10x $$

хитрый прием Учителя:

$$ x^4 = 9 - x^3 - x^2 - x $$

а `x^5` = `x × x^4`

значит

$$ x^5 = x × (9 - x^3 - x^2 - x) $$

а значит:

$$
x^5 - 10x
= x × (9 - x^3 - x^2 - x) - 10x
= 9x - x^4 - x^3 - x^2 - 10x
$$

учитель снова говорит про `x^4 = 9 - x^3 - x^2 - x`:

$$
9x - x^4 - x^3 - x^2 - 10x
= 9x - (9 - x^3 - x^2 - x) - x^3 - x^2 - 10x
= 9x - 9 + x^3 + x^2 + x - x^3 - x^2 - 10x
$$

я продолжаю мысль учителя:

$$
9x - 9 + x - 10x
= 9x - 10x - 9 + x
= -x - 9 + x
= -9
$$
